merkle tree done

theories/ub_logic/merkle_tree.v
@@ -9,8 +9,8 @@ Section merkle_tree.
   Variables val_bit_size':nat.
   Variables max_hash_size : nat.
   Definition val_bit_size : nat := S val_bit_size'.
-  Definition val_size:nat := (2^val_bit_size)-1.
-  Variable (Hineq: (max_hash_size <= val_size)%nat).
+  Definition val_size_for_hash:nat := (2^val_bit_size)-1.
+  Variable (Hineq: (max_hash_size <= val_size_for_hash)%nat).
   Definition leaf_bit_size : nat := 2*val_bit_size.
   (* Definition identifier : nat := 2^leaf_bit_size. *)
   Definition num_of_leafs : nat := 2^height.
@@ -50,30 +50,31 @@ Section merkle_tree.
   Definition map_valid (m:gmap nat Z) : Prop := coll_free m.
   
 
-  Inductive tree_value_match: merkle_tree -> nat -> list bool -> Prop:=
-  | tree_value_match_lf h lf: tree_value_match (Leaf h lf) lf []
-  | tree_value_match_left h l r xs v:
-    tree_value_match l v xs ->
-    tree_value_match (Branch h l r) v (true::xs)
-  | tree_value_match_right h l r xs v:
-    tree_value_match r v xs ->
-    tree_value_match (Branch h l r) v (false::xs).
+  Inductive tree_leaf_value_match: merkle_tree -> nat -> list (bool*nat) -> Prop:=
+  | tree_value_match_lf h lf: tree_leaf_value_match (Leaf h lf) lf []
+  | tree_leaf_value_match_left h l r xs v rhash:
+    tree_leaf_value_match l v xs->
+    tree_leaf_value_match (Branch h l r) v ((true,rhash)::xs)
+  | tree_value_match_right h l r xs v lhash:
+    tree_leaf_value_match r v xs ->
+    tree_leaf_value_match (Branch h l r) v ((false,lhash)::xs).
 
-  Inductive possible_proof: list bool -> list nat -> Prop:=
-  | possible_proof_lf: possible_proof [] []
-  | possible_proof_br b path hashlist hash:
-    possible_proof path hashlist ->
+  (*This ensures all numbers in the proof are smaller than 2^val_bit_size*)
+  Inductive possible_proof: list (bool*nat) -> Prop:=
+  | possible_proof_lf: possible_proof [] 
+  | possible_proof_br b hash prooflist:
+    possible_proof prooflist ->
     hash < 2^val_bit_size ->
-    possible_proof (b::path) (hash::hashlist).
+    possible_proof ((b,hash)::prooflist).
 
-  Inductive correct_proof: merkle_tree -> list bool -> list nat -> Prop :=
-  | correct_proof_lf h l: correct_proof (Leaf h l) [] []
-  | correct_proof_left ltree rtree h path hashlist:
-    correct_proof (ltree) path hashlist ->
-    correct_proof (Branch h ltree rtree) (true::path) (root_hash_value rtree::hashlist)
-  | correct_proof_right ltree rtree h path hashlist:
-    correct_proof (rtree) path hashlist ->
-    correct_proof (Branch h ltree rtree) (false::path) (root_hash_value ltree::hashlist).
+  Inductive correct_proof: merkle_tree -> list (bool*nat) -> Prop :=
+  | correct_proof_lf h l: correct_proof (Leaf h l) []
+  | correct_proof_left ltree rtree h prooflist:
+    correct_proof (ltree) prooflist ->
+    correct_proof (Branch h ltree rtree) ((true, root_hash_value rtree)::prooflist)
+  | correct_proof_right ltree rtree h prooflist:
+    correct_proof (rtree) prooflist ->
+    correct_proof (Branch h ltree rtree) ((false, root_hash_value ltree)::prooflist).
     
 
   Definition root_hash_value_program : val :=
@@ -84,25 +85,20 @@ Section merkle_tree.
       end.
 
   Definition compute_hash_from_leaf : val :=
-    rec: "compute_hash_from_leaf" "ltree" "lhmf" "ll" "lleaf" := 
-    match: "ltree" with
-    | InjL "x" => "lhmf" "lleaf"  
-    | InjR "x"  => let: "b" := (match: list_head "ll" with
-                               | SOME "a" => "a"
-                               | NONE => #()
-                               end
-                              ) in
-                  let: "ll'" := list_tail "ll"  in
-                  let, ("notneeded", "l", "r") := "x" in
-                  if: "b"
-                  then "lhmf"
-                         (("compute_hash_from_leaf" "l" "lhmf" "ll'" "lleaf")*#(2^val_bit_size)+
-                            root_hash_value_program "r")
-                  else "lhmf"
-                         ((root_hash_value_program "l")*#(2^val_bit_size)+("compute_hash_from_leaf" "r" "lhmf" "ll'" "lleaf"))
-    end
-
-  .
+    rec: "compute_hash_from_leaf" "lhmf" "lproof" "lleaf" := 
+       match: list_head "lproof" with
+       | SOME "head" =>
+           let: "lproof'" := list_tail "lproof"  in
+           let, ("b", "hash") := "head" in
+           if: "b"
+           then "lhmf"
+                  (("compute_hash_from_leaf" "lhmf" "lproof'" "lleaf")*#(2^val_bit_size)+
+                "hash")
+           else "lhmf"
+                  ("hash"*#(2^val_bit_size)+("compute_hash_from_leaf" "lhmf" "lproof'" "lleaf"))
+      
+        | NONE => "lhmf" "lleaf"
+        end.
 
   (** Lemmas *)
   Lemma wp_root_hash_value_program n lt tree E:
@@ -128,40 +124,55 @@ Section merkle_tree.
       by eapply lookup_weaken.
   Qed.
 
+  Lemma coll_free_lemma m v v' k:
+    coll_free m -> m!!v=Some k -> m!! v' = Some k -> v= v'.
+  Proof.
+    intros H ? ?.
+    apply H; try done.
+    repeat erewrite lookup_total_correct; try done.
+  Qed.
+
   (** Spec *)
-  Lemma wp_compute_hash_from_leaf_correct (ltree:val) (tree:merkle_tree) (m:gmap nat Z) (v:nat) (path:list bool) llist f E:
+  Lemma wp_compute_hash_from_leaf_correct (ltree:val) (tree:merkle_tree) (m:gmap nat Z) (v:nat) (proof:list (bool*nat)) lproof f E:
      {{{ ⌜tree_relate height ltree tree⌝ ∗
         ⌜tree_valid tree m⌝ ∗
-        hashfun_amortized (val_size-1)%nat max_hash_size f m ∗
-        ⌜is_list path llist⌝ ∗
-        ⌜tree_value_match tree v path⌝ ∗
+        hashfun_amortized (val_size_for_hash)%nat max_hash_size f m ∗
+        ⌜is_list proof lproof⌝ ∗
+        ⌜correct_proof tree proof⌝ ∗
+        ⌜tree_leaf_value_match tree v proof⌝ ∗
         ⌜map_valid m⌝ }}}
-      compute_hash_from_leaf ltree f llist (#v) @ E
+      compute_hash_from_leaf f lproof (#v) @ E
       {{{ (retv:Z), RET #retv;
-          hashfun_amortized (val_size-1) max_hash_size f m ∗
+          hashfun_amortized (val_size_for_hash) max_hash_size f m ∗
           ⌜retv = root_hash_value tree⌝
       }}}.
   Proof.
-    iIntros (Φ) "(%Htrelate&%Htvalid&H&%Hlsit&%Hvmatch&%Hmvalid) HΦ".
-    iInduction tree as [|] "IH"
-                         forall (height ltree v path llist f Htrelate Htvalid Hlsit Hvmatch Hmvalid Φ).
-    - rewrite /compute_hash_from_leaf.
-      wp_pures. inversion Htrelate; subst. 
-      wp_match.
-      inversion Htrelate. inversion Htvalid. inversion Hvmatch. subst.
+    iIntros (Φ) "(%Htrelate & %Htvalid & H & %Hlist & %Hcorrect & %Hvmatch & %Hmvalid) HΦ".
+    iInduction tree as [hash leaf|hash tree1 Htree1 tree2 Htree2] "IH"
+                         forall (height ltree m proof lproof Φ
+                              Htrelate Htvalid Hlist Hcorrect Hvmatch Hmvalid).
+    - rewrite /compute_hash_from_leaf. wp_pures. rewrite -/compute_hash_from_leaf.
+      wp_apply wp_list_head; first done.
+      iIntros (?) "[[-> ->]|%]"; last first.
+      { inversion Hcorrect; subst. destruct H as [?[?[??]]].
+        inversion H. }
+      wp_pures. inversion Htvalid; inversion Hvmatch. subst.
       wp_apply (wp_hashfun_prev_amortized with "[$]").
       + lia.
-      + done. 
-      + iIntros. iApply "HΦ". iFrame. by iPureIntro. 
-    - rewrite /compute_hash_from_leaf.
-      inversion Htrelate. inversion Htvalid. inversion Hvmatch; subst.
-      + wp_pures. wp_apply wp_list_head; first done. iIntros (v') "[[%%]|(%&%&%&%)]"; first done.
-        subst. inversion H; subst. wp_pures. rewrite -/compute_hash_from_leaf.
-        wp_apply wp_list_tail; first done. iIntros (v') "%". wp_pures.
-        wp_apply wp_root_hash_value_program; try done.
-        iIntros (x) "->".
-        wp_apply ("IH" with "[][][][][][H][HΦ]"); try done.
-        iModIntro. iIntros (?) "[H ->]".
+      + done.
+      + iIntros "H". iApply "HΦ"; iFrame.
+        done.
+    - rewrite /compute_hash_from_leaf. wp_pures.
+      rewrite -/compute_hash_from_leaf.
+      wp_apply wp_list_head; first done.
+      iIntros (head) "[[->->]|(%&%&->&->)]".
+      { inversion Hcorrect. }
+      wp_pures. wp_apply wp_list_tail; first done.
+      iIntros (tail) "%Htail".
+      inversion Hcorrect; wp_pures.
+      + inversion Htrelate. inversion Htvalid. inversion Hvmatch; subst; last done.
+        wp_apply ("IH" with "[][][][][][][$]"); try done.
+        iIntros (lhash) "[H ->]".
         wp_pures.
         replace (_*_+_)%Z with (Z.of_nat (root_hash_value tree1 * 2 ^ val_bit_size + root_hash_value tree2)); last first.
         { rewrite Nat2Z.inj_add. f_equal. rewrite Nat2Z.inj_mul. f_equal.
@@ -170,15 +181,11 @@ Section merkle_tree.
         wp_apply (wp_hashfun_prev_amortized with "H").
         * lia.
         * done.
-        * iIntros "H". iApply "HΦ". iFrame.
-          done.
-      + wp_pures. wp_apply wp_list_head; first done. iIntros (v') "[[%%]|(%&%&%&%)]"; first done.
-        subst. inversion H; subst. wp_pures. rewrite -/compute_hash_from_leaf.
-        wp_apply wp_list_tail; first done. iIntros (v') "%". wp_pures.
-        wp_apply ("IH1" with "[][][][][][H][HΦ]"); try done.
-        iModIntro. iIntros (?) "[H ->]".
-        wp_apply wp_root_hash_value_program; try done.
-        iIntros (x) "->".
+        * iIntros "H". iApply "HΦ".
+          iFrame. done.
+      + inversion Htrelate. inversion Htvalid. inversion Hvmatch; subst; first done.
+        wp_apply ("IH1" with "[][][][][][][$]"); try done.
+        iIntros (rhash) "[H ->]".
         wp_pures.
         replace (_*_+_)%Z with (Z.of_nat (root_hash_value tree1 * 2 ^ val_bit_size + root_hash_value tree2)); last first.
         { rewrite Nat2Z.inj_add. f_equal. rewrite Nat2Z.inj_mul. f_equal.
@@ -187,159 +194,169 @@ Section merkle_tree.
         wp_apply (wp_hashfun_prev_amortized with "H").
         * lia.
         * done.
-        * iIntros "H". iApply "HΦ". iFrame.
-          done.
+        * iIntros "H". iApply "HΦ".
+          iFrame. done.
   Qed.
 
-  
-  Lemma wp_compute_hash_from_leaf_incorrect (ltree:val) (tree:merkle_tree) (m:gmap nat Z) (v v':nat) (path:list bool) llist f E:
+  Lemma wp_compute_hash_from_leaf_incorrect (ltree:val) (tree:merkle_tree) (m:gmap nat Z) (v v':nat) (proof:list (bool*nat)) lproof f E:
      {{{ ⌜tree_relate height ltree tree⌝ ∗
         ⌜tree_valid tree m⌝ ∗
-        hashfun_amortized (val_size-1)%nat max_hash_size f m ∗
-        ⌜is_list path llist⌝ ∗
-        ⌜tree_value_match tree v path⌝ ∗
+        hashfun_amortized (val_size_for_hash)%nat max_hash_size f m ∗
+        ⌜is_list proof lproof⌝ ∗
+        ⌜possible_proof proof⌝ ∗
+        ⌜tree_leaf_value_match tree v proof⌝ ∗
+        ⌜v ≠ v'⌝ ∗
         ⌜map_valid m⌝ ∗
         ⌜ size m + (S height) <= max_hash_size⌝ ∗
-        ⌜v ≠ v'⌝ ∗ 
-        € (nnreal_nat (S height) * amortized_error (val_size-1)%nat max_hash_size)%NNR
+        € (nnreal_nat (S height) * amortized_error (val_size_for_hash)%nat max_hash_size)%NNR 
      }}}
-      compute_hash_from_leaf ltree f llist (#v') @ E
+      compute_hash_from_leaf f lproof (#v') @ E
       {{{ (retv:Z), RET #retv;
           ∃ m', ⌜m ⊆ m'⌝ ∗
-                hashfun_amortized (val_size-1) max_hash_size f m' ∗
+                hashfun_amortized (val_size_for_hash) max_hash_size f m' ∗
                 ⌜map_valid m'⌝ ∗
                 ⌜size (m') <= size m + (S height)⌝ ∗
                 ⌜retv ≠ root_hash_value tree⌝ ∗
-                ⌜(0 <= retv)%Z⌝
+                ⌜(0 <= retv < 2^val_bit_size)%Z⌝
       }}}.
   Proof.
-    iIntros (Φ) "(%Htrelate&%Htvalid&H&%Hlsit&%Hvmatch&%Hmvalid&%Hmsize&%Hneq&Herr) HΦ".
+    iIntros (Φ) "(%Htrelate & %Htvalid & H & %Hlist & %Hpossible & %Hvmatch & %Hneq & %Hmvalid & %Hmsize & Herr) HΦ".
     iInduction tree as [|] "IH"
-                         forall (height ltree m path llist Φ Htrelate Htvalid Hlsit Hvmatch Hmvalid Hmsize Hneq).
-    - rewrite /compute_hash_from_leaf.
-      wp_pures. inversion Htrelate; subst. 
-      wp_match.
-      inversion Htrelate. inversion Htvalid. inversion Hvmatch. subst.
-      wp_apply (wp_insert_amortized with "[$H Herr]").
-      + lia.
-      + lia.
-      + iSplitL.
-        * assert (∀ x, (nnreal_nat 1 * x)%NNR = x) as ->; last iFrame.
-          intros. apply nnreal_ext. simpl. lra.
-        * done.
-      + iIntros (v2) "(%m' & Hm & %Hmvalid' & %Hmv' & %Hmsize' & %Hmsubset)".
-        iApply "HΦ". iExists m'.
+                         forall (height ltree m proof lproof Φ Htrelate Htvalid Hlist Hpossible Hvmatch Hmvalid Hmsize).
+    - inversion Htrelate; subst. rewrite /compute_hash_from_leaf. wp_pures.
+      rewrite -/compute_hash_from_leaf. inversion Hvmatch; subst.
+      wp_apply wp_list_head; first done.
+      iIntros (?) "[[_ ->]|(%&%&%&%)]"; last done.
+      wp_pures.
+      wp_apply (wp_insert_amortized with "[$H Herr]"); try lia.
+      + iSplit; try done. iApply ec_spend_irrel; last done.
+        simpl. lra.
+      + iIntros (hash_value') "(%m' & H & %Hvalid' & %Hmfound & %Hmsize' & %Hmsubset)".
+        iApply "HΦ".
+        iExists _.
         repeat iSplit; try done.
-        * iPureIntro. lia.
-        * iPureIntro. simpl. intro Hfalse; subst.
-          apply Hneq. apply Hmvalid'; try done.
-          -- by eapply lookup_weaken_is_Some.
-          -- erewrite lookup_total_correct; last eapply lookup_weaken; try done.
-             by erewrite lookup_total_correct.
-        * iDestruct "Hm" as "(%&%&%&%&%&H)". iPureIntro.
-          eapply map_Forall_lookup_1 in H2; last done.
-          lia. 
-    - rewrite /compute_hash_from_leaf.
-      wp_pures. rewrite -/compute_hash_from_leaf.
+        * iPureIntro; lia.
+        * simpl.
+          inversion Htvalid; subst.
+          iPureIntro. intro; subst. apply Hneq. eapply coll_free_lemma; try done.
+          by erewrite lookup_weaken.
+        * rewrite /hashfun_amortized. iDestruct "H" as "(%&%&%&%&%Hforall&H)".
+          iPureIntro. eapply map_Forall_lookup_1 in Hforall; last done.
+          lia.
+        * rewrite /hashfun_amortized. iDestruct "H" as "(%&%&%&%&%Hforall&H)".
+          iPureIntro. eapply map_Forall_lookup_1 in Hforall; last done. 
+          rewrite /val_size_for_hash in Hforall. destruct Hforall as [? H1].
+          apply Zle_lt_succ in H1.
+          eapply Z.lt_stepr; try done.
+          rewrite -Nat2Z.inj_succ. replace (2)%Z with (Z.of_nat 2) by lia.
+          rewrite -Nat2Z.inj_pow. f_equal.
+          assert (1<=2 ^val_bit_size); last lia. clear.
+          induction val_bit_size; simpl; lia.
+    - rewrite /compute_hash_from_leaf. wp_pures. rewrite -/compute_hash_from_leaf.
+      wp_apply wp_list_head; first done.
+      iIntros (?) "[[->->]|(%head & %lproof' & -> & ->)]".
+      { inversion Hvmatch. }
+      wp_pures. wp_apply wp_list_tail; first done.
+      iIntros (proof') "%Hproof'".
+      wp_pures. inversion Hpossible; subst.
+      wp_pures.
       inversion Htrelate; subst.
-      wp_pures. inversion Htvalid; subst.
-      inversion Hvmatch; subst.
-      + wp_apply wp_list_head; try done. iIntros (?) "[%|%Hl]".
-        { naive_solver. }
-        destruct Hl as (?&?&?&?); subst. inversion H; subst.
+      iAssert (€ ((nnreal_nat (S n) * amortized_error val_size_for_hash max_hash_size)%NNR) ∗
+               € (amortized_error val_size_for_hash max_hash_size)%NNR)%I with "[Herr]" as "[Herr Herr']".
+      { iApply ec_split. iApply (ec_spend_irrel with "[$]").
+        simpl. lra.
+      }
+      inversion Hvmatch; inversion Htvalid; subst; wp_pures.
+      + wp_apply ("IH" with "[][][][][][][][$H][$Herr]"); try done.
+        { iPureIntro; lia. }
+        iIntros (lefthash') "(%m' & %Hmsubset & H & %Hmvalid' & %Hmsize' & %Hlefthashneq & %Hlefthashsize')".
         wp_pures.
-        wp_apply wp_list_tail; try done.
-        iIntros (l') "%".
+        replace (_*_+_)%Z with (Z.of_nat (Z.to_nat lefthash' * 2 ^ val_bit_size + hash)); last first.
+        { rewrite Nat2Z.inj_add. f_equal. rewrite Nat2Z.inj_mul.
+          rewrite Z2Nat.id; last lia. f_equal.
+          rewrite Z2Nat.inj_pow. f_equal.
+        } 
+        wp_apply (wp_insert_amortized with "[$H $Herr']").
+        * lia.
+        * lia.
+        * by iPureIntro.
+        * iIntros (finalhash) "(%m'' & H & %Hmvalid'' & %Hmfound'' & %Hmsize'' & %Hmsubset')".
+          iApply "HΦ".
+          iExists m''. repeat iSplit.
+          -- iPureIntro; etrans; exact.
+          -- done.
+          -- by iPureIntro.
+          -- iPureIntro; lia.
+          -- iPureIntro. simpl.
+             intro; subst. apply Hlefthashneq.
+             assert (root_hash_value tree1 * 2 ^ val_bit_size + root_hash_value tree2 =
+                     Z.to_nat lefthash' * 2 ^ val_bit_size + hash) as helper.
+             { eapply (coll_free_lemma m''); try done.
+               eapply lookup_weaken; first done.
+               etrans; exact.
+             }
+             epose proof (Nat.mul_split_l _ _ _ _ _ _ _ helper) as [Hsplit _].
+             lia.
+             Unshelve.
+             ++ by inversion H15.
+             ++ by inversion Hpossible. 
+          -- rewrite /hashfun_amortized. iDestruct "H" as "(%&%&%&%&%Hforall&H)".
+             iPureIntro. eapply map_Forall_lookup_1 in Hforall; last done. lia.
+          -- rewrite /hashfun_amortized. iDestruct "H" as "(%&%&%&%&%Hforall&H)".
+             iPureIntro. eapply map_Forall_lookup_1 in Hforall; last done. 
+             rewrite /val_size_for_hash in Hforall. destruct Hforall as [? H3].
+             apply Zle_lt_succ in H3.
+             eapply Z.lt_stepr; try done.
+             rewrite -Nat2Z.inj_succ. replace (2)%Z with (Z.of_nat 2) by lia.
+             rewrite -Nat2Z.inj_pow. f_equal.
+             assert (1<=2 ^val_bit_size); last lia. clear.
+             induction val_bit_size; simpl; lia.        
+      + wp_apply ("IH1" with "[][][][][][][][$H][$Herr]"); try done.
+        { iPureIntro; lia. }
+        iIntros (righthash') "(%m' & %Hmsubset & H & %Hmvalid' & %Hmsize' & %Hrighthashneq & %Hrighthashsize')".
         wp_pures.
-        wp_apply wp_root_hash_value_program; try done.
-        iIntros (?) "->".
-        iAssert (€ ((nnreal_nat (S n) * amortized_error (val_size - 1) max_hash_size)%NNR) ∗
-                 € (amortized_error (val_size - 1) max_hash_size)%NNR)%I with "[Herr]" as "[Herr Herr']".
-        { iApply ec_split. iApply (ec_spend_irrel with "[$]").
-          simpl. lra.
-        }
-        wp_apply ("IH" with "[][][][][][][][$H][$Herr]"); try done.
-        * iPureIntro. lia. 
-        * iIntros (retv) "(%m' & %Htvalid' & H & %Hmvalid' & %Hmsize' & %Hneq' & %Hnonneg)".
-          wp_pures.
-          replace (_*_+_)%Z with (Z.of_nat (Z.to_nat retv * 2 ^ val_bit_size + root_hash_value tree2)); last first.
-          { rewrite Nat2Z.inj_add. f_equal. rewrite Nat2Z.inj_mul. f_equal; first lia.
-            apply Z2Nat.inj_pow.
-          }
-          wp_apply (wp_insert_amortized with "[$H $Herr']").
-          -- lia.
-          -- lia.
-          -- iPureIntro. done.
-          -- iIntros (hv) "(%m''&Hm'' & %Hcoll_free' & %Hmsome'' & %Hsize'' & %Hsubset'')".
-             iApply "HΦ".
-             iExists m''.
-             repeat iSplit; try done.
-             ++ iPureIntro. etrans; exact.
-             ++ iPureIntro. lia.
-             ++ simpl. iPureIntro.
-                intro; subst. apply Hneq'.
-                assert (Z.to_nat retv * 2 ^ val_bit_size + root_hash_value tree2 =
-                        root_hash_value tree1 * 2 ^ val_bit_size + root_hash_value tree2); last first.
-                { assert (Z.to_nat retv =
-                          root_hash_value tree1 ); try lia.
-                  assert (Z.to_nat retv * 2 ^ val_bit_size =
-                          root_hash_value tree1 * 2 ^ val_bit_size); try lia.
-                  rewrite <- Nat.mul_cancel_r; try done.
-                  lia.
-                }
-                apply Hcoll_free'; try done.
-                ** eapply lookup_weaken_is_Some; try done.
-                   etrans; exact.
-                ** erewrite lookup_total_correct; last done.
-                   erewrite lookup_total_correct; last eapply lookup_weaken; try done.
-                   etrans; exact.
-             ++ iDestruct "Hm''" as "(%&%&%&%&%&%&H)".
-                iPureIntro. eapply map_Forall_lookup_1 in H6; last done. lia.
-      + wp_apply wp_list_head; try done. iIntros (?) "[%|%Hl]".
-        { naive_solver. }
-        destruct Hl as (?&?&?&?); subst. inversion H; subst.
-        wp_pures.
-        wp_apply wp_list_tail; try done.
-        iIntros (l') "%".
-        wp_pures.
-        iAssert (€ ((nnreal_nat (S n) * amortized_error (val_size - 1) max_hash_size)%NNR) ∗
-                 € (amortized_error (val_size - 1) max_hash_size)%NNR)%I with "[Herr]" as "[Herr Herr']".
-        { iApply ec_split. iApply (ec_spend_irrel with "[$]").
-          simpl. lra.
-        }
-        wp_apply ("IH1" with "[][][][][][][][$H][$Herr]"); try done.
-        * iPureIntro. lia.
-        * iIntros (retv) "(%m' & %Htvalid' & H & %Hmvalid' & %Hmsize' & %Hneq' & %Hnonneg)".
-          wp_pures.
-          wp_apply wp_root_hash_value_program; try done.
-          iIntros (?) "->".
-          wp_pures.
-          replace (_*_+_)%Z with (Z.of_nat ((root_hash_value tree1) * 2 ^ val_bit_size + Z.to_nat retv)); last first.
-          { rewrite Nat2Z.inj_add. f_equal; try lia. rewrite Nat2Z.inj_mul. f_equal. 
-            apply Z2Nat.inj_pow.
-          }
-          wp_apply (wp_insert_amortized with "[$H $Herr']").
-          -- lia.
-          -- lia.
-          -- iPureIntro. done.
-          -- iIntros (hv) "(%m''&Hm'' & %Hcoll_free' & %Hmsome'' & %Hsize'' & %Hsubset'')".
-             iApply "HΦ".
-             iExists m''.
-             repeat iSplit; try done.
-             ++ iPureIntro. etrans; exact.
-             ++ iPureIntro. lia.
-             ++ simpl. iPureIntro.
-                intro; subst. apply Hneq'.
-                assert (root_hash_value tree1 * 2 ^ val_bit_size + Z.to_nat retv =
-                        root_hash_value tree1 * 2 ^ val_bit_size + root_hash_value tree2); try lia.
-                apply Hcoll_free'; try done.
-                ** eapply lookup_weaken_is_Some; try done.
-                   etrans; exact.
-                ** erewrite lookup_total_correct; last done.
-                   erewrite lookup_total_correct; last eapply lookup_weaken; try done.
-                   etrans; exact.
-             ++ iDestruct "Hm''" as "(%&%&%&%&%&%&H)".
-                iPureIntro. eapply map_Forall_lookup_1 in H6; last done. lia.
+        replace (_*_+_)%Z with (Z.of_nat (hash * 2 ^ val_bit_size + Z.to_nat righthash')); last first.
+        { rewrite Nat2Z.inj_add. f_equal; last lia. rewrite Nat2Z.inj_mul. f_equal.
+          rewrite Z2Nat.inj_pow. f_equal.
+        } 
+        wp_apply (wp_insert_amortized with "[$H $Herr']").
+        * lia.
+        * lia.
+        * by iPureIntro.
+        * iIntros (finalhash) "(%m'' & H & %Hmvalid'' & %Hmfound'' & %Hmsize'' & %Hmsubset')".
+          iApply "HΦ".
+          iExists m''. repeat iSplit.
+          -- iPureIntro; etrans; exact.
+          -- done.
+          -- by iPureIntro.
+          -- iPureIntro; lia.
+          -- iPureIntro. simpl.
+             intro; subst. apply Hrighthashneq.
+             assert (root_hash_value tree1 * 2 ^ val_bit_size + root_hash_value tree2 =
+                     hash * 2 ^ val_bit_size + Z.to_nat righthash') as helper.
+             { eapply (coll_free_lemma m''); try done.
+               eapply lookup_weaken; first done.
+               etrans; exact.
+             }
+             epose proof (Nat.mul_split_l _ _ _ _ _ _ _ helper) as [Hsplit _].
+             lia.
+             Unshelve.
+             ++ by inversion H15.
+             ++ destruct Hrighthashsize' as [Hrighthashsize Hrighthashsize'].
+                rewrite Nat2Z.inj_lt. rewrite Z2Nat.inj_pow.
+                replace (Z.of_nat 2) with 2%Z by lia.
+                rewrite Z2Nat.id; lia.
+          -- rewrite /hashfun_amortized. iDestruct "H" as "(%&%&%&%&%Hforall&H)".
+             iPureIntro. eapply map_Forall_lookup_1 in Hforall; last done. lia.
+          -- rewrite /hashfun_amortized. iDestruct "H" as "(%&%&%&%&%Hforall&H)".
+             iPureIntro. eapply map_Forall_lookup_1 in Hforall; last done. 
+             rewrite /val_size_for_hash in Hforall. destruct Hforall as [? H3].
+             apply Zle_lt_succ in H3.
+             eapply Z.lt_stepr; try done.
+             rewrite -Nat2Z.inj_succ. replace (2)%Z with (Z.of_nat 2) by lia.
+             rewrite -Nat2Z.inj_pow. f_equal.
+             assert (1<=2 ^val_bit_size); last lia. clear.
+             induction val_bit_size; simpl; lia. 
   Qed.
   
   
